WIP

bst_inst.v
@@ -1,124 +1,172 @@
 Require Import VST.concurrency.conclib.
+From iris.algebra Require Import excl auth gmap agree gset.
+Require Import flows.inset_flows.
+Require Import flows.auth_ext.
+Require Import flows.multiset_flows.
+Require Import flows.flows.
+Require Import iris_ora.algebra.gmap.
+Require Import iris_ora.logic.own.
+Require Import iris_ora.algebra.ext_order.
+Require Import iris_ora.algebra.frac_auth.
 Require Import VST.floyd.proofauto.
 Require Import VST.atomics.general_locks.
-Require Import bst.puretree.
-Require Import bst.bst.
-Require Import bst.data_struct.
-Require Import VST.atomics.verif_lock_atomic.
 Require Import VST.floyd.library.
+Require Import VST.atomics.verif_lock_atomic.
+Require Import tmpl.puretree.
+Require Import tmpl.bst. (*binary search tree*)
+Require Import tmpl.keyset_ra_ora.
+Require Import tmpl.puretree.
+Require Import tmpl.data_struct.
+Require Import tmpl.flows_ora.
+
 
 #[export] Instance CompSpecs : compspecs. make_compspecs prog. Defined.
 Definition Vprog : varspecs.  mk_varspecs prog. Defined.
 
-(* struct node {int key; void *value; struct tree_t *left, *right;} node;*)
-Definition t_struct_tree := Tstruct _node noattr.
-(* Define for dynamic list *)
-Definition struct_dlist := Tstruct _DList noattr.
+#[global] Instance gmap_inhabited V : Inhabitant (gmap key V).
+Proof. unfold Inhabitant; apply empty. Defined.
+
+#[global] Instance number_inhabited: Inhabitant number.
+Proof. unfold Inhabitant; apply Pos_Infinity. Defined.
+
+Section give_up_traverse.
+  Context `{N: NodeRep } `{EqDecision K} `{Countable K}.
+  Context `{!VSTGS unit Σ, !cinvG Σ, atom_impl : !atomic_int_impl (Tstruct _atom_int noattr),
+            !flowintG Σ, !nodesetG Σ, !keysetG Σ, !keymapG Σ, inG Σ (frac_authR (agreeR Node))}.
+
+  (* struct node {int key; void *value; struct tree_t *left, *right;} node;*)
+  Definition t_struct_tree := Tstruct _node noattr.
+  (* Define for dynamic list *)
+  Definition struct_dlist := Tstruct _DList noattr.
 
 (* struct tree_t {node *t; lock_t *lock; int min; int max; } tree_t; *)
 (* Definition t_struct_tree_t := Tstruct _tree_t noattr. *)
 
 (* node_rep_R r.1.1.1 r.1.2 r.2 g, and r is type of node_info *)
 
+(*
+Class NodeRep : Type := {
+    node : val → @multiset_flowint_ur Key _ _ → gmap Key Value -> gmap nat Node -> mpred;
+    (* node_sep_star: ∀ n I_n I_n' C C', node n I_n C ∗ node n I_n' C' -∗ False; *)
+    node_rep_R_valid_pointer: forall n I_n C next, node n I_n C next -∗ valid_pointer n;
+    node_rep_R_pointer_null: forall n I_n C next, node n I_n C next -∗ ⌜is_pointer_or_null n⌝;
+    node_size: nat;
+}.
 
+ *)
+
+ Check list Node.
+
+
+  
 #[local] Obligation Tactic := idtac.
 
 #[local] Program Instance my_specific_tree_rep : NodeRep := {
-  node_rep_R := fun (tp : val) (r : range) (g_info : option (option ghost_info)) g =>
-  if eq_dec tp nullval
-  then !!(g_info = Some None) && seplog.emp
+  node := fun (n : Node) (In : @multiset_flowint_ur Key _ _) (C: gmap Key data_struct.Value)
+            (next:  gmap nat Node) =>
+  if eq_dec n nullval
+  then ⌜True⌝
   else
-  (EX (x : Z), EX (v pa pb : val),
-      !!(g_info = Some (Some (x, v, [pa; pb])) /\ and (Z.le Int.min_signed x) (Z.le x Int.max_signed) /\
-       is_pointer_or_null pa /\ is_pointer_or_null pb /\
-          (tc_val (tptr Tvoid) v) /\ key_in_range x r = true) &&
-       data_at Ews t_struct_tree ((Vint (Int.repr x)), (v, (pa, pb))) tp * 
-       malloc_token Ews t_struct_tree tp); node_size := 2}.
+  (∃ (x : Z) (v : val) (p1 p2: nat),
+      ⌜and (Z.le Int.min_signed x) (Z.le x Int.max_signed) /\
+       is_pointer_or_null (next !!! p1) /\ is_pointer_or_null (next !!! p2) /\
+          (tc_val (tptr Tvoid) v) ∧
+        (forall y, in_outset _ _ _ y In (next !!! p1) <-> Z.lt y x ∧ in_inset _ _ _ y In n) ∧
+        (forall y, in_outset _ _ _ y In (next !!! p2) <-> Z.lt x y ∧ in_inset _ _ _ y In n) ∧
+        (forall y, in_outsets _ _ _ y In -> in_outset _ _ _ y In (next !!! p1) ∨ in_outset _ _ _ y In (next !!! p2))⌝ ∧
+       data_at Ews t_struct_tree (Vint (Int.repr x), (v, ((next !!! p1), (next !!! p2)))) n ∗
+       malloc_token Ews t_struct_tree n); node_size := 2}.
 (* ; node_rep_R_valid_pointer }. *)
 Next Obligation.
-  simpl.
-  intros tp r g_info g.
-  destruct (EqDec_val tp nullval); [ | Intros x v pa pb]; entailer !.
+  intros n In Cn next. 
+  destruct (EqDec_val n nullval). 
+  - simpl. rewrite e. auto.
+  - rewrite if_false; auto. iIntros "H".
+    iDestruct "H" as (x v p1 p2) "(%HJ & (H1 & H2))".
+    iStopProof. entailer !.
 Defined.
 Next Obligation.
-  simpl.
-  intros tp r g_info g.
-  destruct (EqDec_val tp nullval); [ | Intros x v pa pb]; entailer !.
+  intros n In Cn next.
+  destruct (EqDec_val n nullval).
+  - simpl. rewrite e. auto.
+  - rewrite if_false; auto.
+    iIntros "H".
+    iDestruct "H" as (x v p1 p2) "(%HJ & (H1 & H2))".
+    iStopProof. entailer !.
 Defined.
-
-Definition extract_node_pn (node: node_info) : list val :=
-  match node.2 with
-  | Some (Some (_, _, lst)) => lst
-  | _ => []
-  end.
 
 (* Spec of findnext function *)
 (* FOUND = 0, NOTFOUND = 1, NULLNEXT = 2 (NULLNEXT = NULL || NEXT ) *)
 Definition findnext_spec :=
   DECLARE _findNext
-  WITH x: Z, p: val, n: val, n_pt : val, r: node_info,
-                g: gname, sh: share, gv: globals
+  WITH x: Z, p: Node, n: val, n_pt : val, Ip : flowintT,
+                Cp : (gmap Key data_struct.Value), nextp : gmap nat Node, sh: share, gv: globals
   PRE [ tptr t_struct_tree, tptr (tptr tvoid), tint ]
-          PROP (writable_share sh(*; is_pointer_or_null pa; is_pointer_or_null pb*) )
+          PROP (writable_share sh;
+                (Int.min_signed ≤ x ≤ Int.max_signed)%Z
+          (*; is_pointer_or_null pa; is_pointer_or_null pb*) )
           PARAMS (p; n; Vint (Int.repr x)) GLOBALS (gv)
-          SEP (node_rep_R r.1.1.1 r.1.2 r.2 g * (!!(p = r.1.1.1 /\ p <> nullval) && seplog.emp) *
+          SEP (node p Ip Cp nextp ∗ ⌜p <> nullval /\ in_inset _ _ _ x Ip p⌝ ∧
                (* field_at sh (t_struct_tree) [StructField _t] r.1.1.1 p; *)
                data_at sh (tptr tvoid) n_pt n)
   POST [ tint ]
-  EX (stt: enum), EX (n' next : val),
+  ∃ (stt: enum), ∃ (n' next : Node),
          PROP (match stt with
                | F | NF => (n' = p)
                | NN => (n' = next)
                end)
         LOCAL (temp ret_temp (enums stt))
         SEP (match stt with
-               | F | NF => data_at sh (tptr tvoid) n_pt n
-               | NN => !!(n' ∈ extract_node_pn r) && data_at sh (tptr tvoid) next n
-             end *
-               node_rep_R r.1.1.1 r.1.2 r.2 g) .
-
+               | F | NF => ⌜¬in_outsets _ _ _ x Ip⌝ ∧ data_at sh (tptr tvoid) n_pt n
+               | NN => ⌜in_outset _ _ _ x Ip next⌝ ∧ data_at sh (tptr tvoid) next n
+             end ∗
+               node p Ip Cp nextp).
 
 Lemma findNext: semax_body Vprog Gprog f_findNext findnext_spec.
 Proof.
   start_function.
-  unfold node_rep_R.
-  unfold my_specific_tree_rep.
   Intros.
-  subst.
+  unfold node.
+  unfold my_specific_tree_rep.
   rewrite -> if_false; eauto.
-  Intros x0 v0 pa pb.
+  Intros x0 v0 p1 p2.
   forward.
   forward_if. (* if (_x < _y) *)
   - forward. forward. forward.
-    Exists NN pa pa.
+    Exists NN (nextp !!! p1) (nextp !!! p1) .
+    unfold node.
+    unfold my_specific_tree_rep.
+    rewrite -> if_false; auto.
+    Exists x0 v0 p1 p2.
     entailer !.
-    unfold extract_node_pn.
-    rewrite H.
-    apply elem_of_list_here.
-    rewrite H.
-    simpl.
-    rewrite -> if_false; eauto.
-    Exists x0 v0 pa pb.
-    entailer !.
-  - forward_if.
+    apply (H8 x). split. lia.
+    auto.
+  - (* if (_x > _y) *)
+    forward_if.
     repeat forward.
-    Exists NN pb pb.
+    Exists NN (nextp !!! p2) (nextp !!! p2).
     entailer !.
-    unfold extract_node_pn.
-    rewrite H. simpl.
-    assert([pa ; pb] = [pa] ++ [pb]) as K by auto.
-    rewrite K elem_of_app; right; apply elem_of_list_here. 
-    simpl.
-    rewrite -> if_false; eauto.
-    Exists x0 v0 pa pb.
+    apply (H9 x). split. lia. auto. 
+    unfold node, my_specific_tree_rep.
+    rewrite -> if_false; auto.
+    Exists x0 v0 p1 p2.
     entailer !.
+    (* x = y *)
     forward.
-    Exists F r.1.1.1  n_pt.
+    Exists F p p.
+    unfold node, my_specific_tree_rep.
+    rewrite -> if_false; auto.
+    Exists x0 v0 p1 p2.
     entailer !.
-    simpl.
-    rewrite -> if_false; eauto.
-    Exists x0 v0 pa pb.
-    entailer !.
+    assert (x = x0). lia.
+    subst x0.
+    specialize (H8 x).
+    specialize (H9 x).
+    specialize (H10 x).
+    apply H10 in H18.
+    destruct H18.
+    apply H8 in H18. lia.
+    apply H9 in H18. lia.
 Qed.
 
 Definition surely_malloc_spec :=
@@ -131,10 +179,10 @@ Definition surely_malloc_spec :=
        PARAMS (Vptrofs (Ptrofs.repr (sizeof t))) GLOBALS (gv)
        SEP (mem_mgr gv)
     POST [ tptr tvoid ]
-    EX p: _,
+    ∃ p: _,
        PROP ()
        RETURN (p)
-       SEP (mem_mgr gv; malloc_token Ews t p * data_at_ Ews t p).
+       SEP (mem_mgr gv; malloc_token Ews t p ∗ data_at_ Ews t p).
 
 Definition insertOp_spec :=
   DECLARE _insertOp
@@ -151,7 +199,7 @@ Definition insertOp_spec :=
                      (* (!!(p = r.1.1.1 /\ p = nullval)  && seplog.emp); *)
        data_at Ews (tptr t_struct_tree) tp p)
   POST[ tvoid ]
-  EX (pnt : val),
+  ∃ (pnt : val),
   PROP (pnt <> nullval)
   LOCAL ()
   SEP (mem_mgr gv; data_at Ews (tptr t_struct_tree) pnt p;
