data_struct.v
@@ -18,12 +18,11 @@ Require Import tmpl.giveup_template.
 Require Import tmpl.keyset_ra_ora.
 
 Definition Key := Z.
+Definition Value := val.
 
 Section Give_Up_Cameras.
   Lemma flwint n (x y : @multiset_flowint_ur Key _ _): ✓{n} y → x ≼ₒ{n} y → x ≼{n} y.
-    Proof.
-      intros Hv Hxy; destruct y; destruct Hxy; subst; try done.
-    Qed.
+  Proof. intros Hv Hxy; destruct y; destruct Hxy; subst; try done. Qed.
   Canonical Structure flow_authR := @authR _ flwint.
 
   (* RA for authoritative flow interfaces over multisets of keys *)
@@ -34,6 +33,21 @@ Section Give_Up_Cameras.
   Proof. solve_inG. Qed.
 
   (* RA for authoritative sets of nodes *)
+
+  Canonical Structure gmap_authR K A `{Countable K} :=
+    inclR(iris.algebra.auth.authR(iris.algebra.gmap.gmapR K A)).
+
+  Locate agree.
+  Check iris.algebra.agree.agree.
+  Class nodemapG Σ := NodesetG { nodemap_inG :> inG Σ (gmap_authR Node (iris.algebra.agree.agree (prodO val val))) }.
+  Definition nodemapΣ : gFunctors := #[GFunctor (gmap_authR Node (iris.algebra.agree.agree (prodO val val)))].
+
+  Locate agree.
+
+  Instance subG_nodemapΣ {Σ} : subG nodemapΣ Σ → nodemapG Σ.
+  Proof. solve_inG. Qed.
+
+(*
   
   Canonical Structure gset_authR A `{Countable A} := inclR(iris.algebra.auth.authR(gsetR A)).
 
@@ -42,16 +56,42 @@ Section Give_Up_Cameras.
 
   Instance subG_nodesetΣ {Σ} : subG nodesetΣ Σ → nodesetG Σ.
   Proof. solve_inG. Qed.
+*)
 
-  Lemma ks A `{Countable A} n  (x y : keysetUR A): ✓{n} y → x ≼ₒ{n} y → x ≼{n} y.
+  (* keymap *)
+
+  Canonical Structure keymap_authR K A `{Countable K} :=
+    inclR(iris.algebra.auth.authR(iris.algebra.gmap.gmapR K A)).
+
+  Class keymapG Σ := KeymapG { keymap_inG :>
+                                 inG Σ (keymap_authR Key (iris.algebra.excl.exclR (discreteO val)))}.
+  Definition keymapΣ : gFunctors :=
+    #[GFunctor (keymap_authR Key (iris.algebra.excl.exclR (discreteO val)))].
+
+  Instance subG_keymapΣ {Σ} : subG (@keymapΣ) Σ → (@keymapG) Σ.
+  Proof. solve_inG. Qed.
+  
+  Lemma ks A `{Countable A} n (x y : keysetUR A): ✓{n} y → x ≼ₒ{n} y → x ≼{n} y.
   Proof. intros Hv Hxy; destruct y; destruct Hxy; subst; try done. Qed.
   Canonical Structure keyset_authR A `{Countable A} := @authR _ (ks A).
 
-  Class keysetG Σ := KeysetG { keyset_inG :> inG Σ (keyset_authR Key  ) }.
+  Class keysetG Σ := KeysetG { keyset_inG :> inG Σ (keyset_authR Key) }.
   Definition keysetΣ : gFunctors := #[GFunctor (keyset_authR Key)].
 
   Instance subG_keysetΣ {Σ} : subG (@keysetΣ) Σ → (@keysetG) Σ.
   Proof. solve_inG. Qed.
+  
+
+  (*
+  Canonical Structure gmap_authR K `{Countable K} A := inclR(iris.algebra.auth.authR(iris.algebra.gmap.gmapR K A )).
+
+  Class nodemapG Σ := NodemapG { nodemap_inG :> inG Σ (gmap_authR Key Node) }.
+  Definition nodesetΣ : gFunctors := #[GFunctor (gset_authR Node )].
+
+  Instance subG_nodesetΣ {Σ} : subG nodesetΣ Σ → nodesetG Σ.
+  Proof. solve_inG. Qed.
+*)
+  
 End Give_Up_Cameras.
 
 Definition number2Z (x : number) : Z :=
@@ -72,48 +112,50 @@ Definition enums x : val :=
   | NN => Vint (Int.repr 2%Z)
   end.
 
-#[global] Instance enum_inhabited : Inhabitant (enum).
-Proof.
-  unfold Inhabitant; apply F.
-Defined.
+#[global] Instance enum_inhabited : Inhabitant enum.
+Proof. unfold Inhabitant; apply F. Defined.
 
-Definition pointer_of (n : Node) :=  fst n.
+(* Definition pointer_of (n : Node) :=  fst n.
 Definition lock_of (n : Node) := fst (snd n).
 Definition node_of (n : Node) := snd (snd n).
+*)
 Definition min_of (rg: (number * number)) := fst rg.
 Definition max_of (rg: (number * number)) := snd rg.
 
-
+(*Node = val.
+gmap Node -> (val, val) 
+ *)
 Section NodeRep.
-Context `{!VSTGS unit Σ, !flowintG Σ, !nodesetG Σ, !keysetG Σ }.
+Context `{!VSTGS unit Σ, !flowintG Σ, !nodemapG Σ, !keymapG Σ }.
+
+Definition inFP (γ_f: gname) (pn lock: val) (n : Node) : mpred :=
+    ∃ (N: gmap Node (val * val)),
+      own (inG0 := nodemap_inG) γ_f (◯ (to_agree <$> N) : gmap_authR Node _) ∧
+        ⌜N !! n = Some (pn, lock)⌝.
+
+(*
 Definition inFP (γ_f: gname) (n : Node) : mpred :=
     ∃ (N: gset Node),
       (own (inG0 := nodeset_inG)) γ_f (◯ N : gset_authR _) ∧ ⌜n ∈ N⌝.
+*)
 
 Class NodeRep : Type := {
-    node : Node → @multiset_flowint_ur Key _ _ → gset Key → mpred;
-    (* node_sep_star: ∀ n I_n I_n' C C', node n I_n C ∗ node n I_n' C' -∗ False; *)
-    node_rep_R_valid_pointer: forall n I_n C, node n I_n C -∗ valid_pointer (pointer_of n);
-    node_rep_R_pointer_null: forall n I_n C, node n I_n C -∗ ⌜is_pointer_or_null (pointer_of n)⌝;
+    node : Node → @multiset_flowint_ur Key _ _ → gmap Key Value -> gmap nat Node -> mpred;
+    node_rep_R_valid_pointer: forall n I_n C next, node n I_n C next -∗ valid_pointer n;
+    node_rep_R_pointer_null: forall n I_n C next, node n I_n C next -∗ ⌜is_pointer_or_null n⌝;
     node_size: nat;
 }.
 
-Global Instance inFP_persistent γ_f n: Persistent (inFP γ_f n).
+Global Instance inFP_persistent γ_f pn lock n: Persistent (inFP γ_f pn lock n).
 Proof.
   apply bi.exist_persistent.
   intros x.
   apply bi.and_persistent.
   apply own_core_persistent.
   apply (iris.algebra.auth.auth_frag_core_id _ ).
-  apply _. apply _.
+  apply _.
+  apply _.
 Qed.
 
 End NodeRep.
 
-#[export] Instance CompSpecs : compspecs. make_compspecs prog. Defined.
-Definition Vprog : varspecs.  mk_varspecs prog. Defined.
-
-
-(*
-
-*)
