giveup_lib.v
@@ -21,11 +21,16 @@ Require Import tmpl.data_struct.
 #[export] Instance CompSpecs : compspecs. make_compspecs prog. Defined.
 Definition Vprog : varspecs.  mk_varspecs prog. Defined.
 
+Definition Value := iris.algebra.excl.exclR (discreteO val).
 
 Section give_up.
   Context `{N: NodeRep } `{EqDecision K} `{Countable K}.
-  Context `{!VSTGS OK_ty Σ, !cinvG Σ, atom_impl : !atomic_int_impl (Tstruct _atom_int noattr),
-            !flowintG Σ, !nodesetG Σ, !keysetG Σ, inG Σ (frac_authR (agreeR Node))}.
+   
+  Definition prod3O A B C D E := prodO A (prodO B (prodO C (prodO D E))).
+  Definition per_node := prod3O val val Node (@multiset_flowint_ur Key _ _) (gmap Key data_struct.Value).
+  Context `{!VSTGS unit Σ, !cinvG Σ, atom_impl : !atomic_int_impl (Tstruct _atom_int noattr),
+            !flowintG Σ, !nodemapG Σ, !keymapG Σ, !keysetG Σ,
+        inG Σ (frac_authR (agreeR per_node))}.
   
   Definition t_struct_node := Tstruct _node_t noattr.
   Definition t_struct_nodeds := Tstruct _node noattr.
@@ -34,16 +39,29 @@ Section give_up.
   (* struct node_t {node *t; lock_t lock; int min; int max; } node_t;
     struct node {int key; void *value; void *left, *right;} node; *)
 
-  Definition node_rep γ_f γ_k (n : Node) (rg : (number * number))
-    (In : @multiset_flowint_ur Key _ _ ) Cn :=
+  
+
+  Lemma inFP_duplicate γ_f pn lock n:
+    inFP γ_f pn lock n -∗ inFP γ_f pn lock n ∗ inFP γ_f pn lock n.
+  Proof. by rewrite - bi.persistent_sep_dup; iIntros "?". Qed.
+
+  (* γ_f for N: gset Node)
+    γ_I for In (multiset_flowint_ur)
+    γ_k for keyset 
+   *)
+  
+  Definition node_rep γ_I γ_k pn lock (n : Node)
+    (In : @multiset_flowint_ur Key _ _ ) Cn := ∃ (rg : (number * number)) next,
     ⌜repable_signed (number2Z (min_of rg)) ∧ repable_signed (number2Z (max_of rg)) /\
-      is_pointer_or_null (node_of n) /\ is_pointer_or_null (lock_of n)⌝ ∧
-      field_at Ews (t_struct_node) [StructField _t] (node_of n) (pointer_of n) ∗ (* pn ->n*) 
-      field_at Ews (t_struct_node) [StructField _min] (vint (number2Z (min_of rg))) (pointer_of n) ∗ (*pn -> min*)
-      field_at Ews (t_struct_node) [StructField _max] (vint (number2Z (max_of rg))) (pointer_of n) ∗ (*pn -> max*) 
-      malloc_token Ews t_struct_node (pointer_of n) (* ∗ inFP γ_f n *) ∗
-      node n In Cn ∗ own γ_k (◯ prod (keyset _ _ Key In n, Cn): keyset_authR Key) ∗
-      own γ_f (◯ In) ∗ ⌜dom In = {[n]}⌝.
+      is_pointer_or_null n /\ is_pointer_or_null lock ∧
+      (∀ k, and (Z.lt (number2Z (min_of rg)) k) (Z.lt k (number2Z (max_of rg))) -> in_inset _ _ _ k In n) ∧ dom In = {[n]} ⌝ ∧
+      field_at Ews (t_struct_node) [StructField _t] n pn ∗ (* pn ->n*) 
+      field_at Ews (t_struct_node) [StructField _min] (vint (number2Z (min_of rg))) pn ∗ (*pn -> min*)
+      field_at Ews (t_struct_node) [StructField _max] (vint (number2Z (max_of rg))) pn ∗ (*pn -> max*)
+      
+      malloc_token Ews t_struct_node pn (* ∗ inFP γ_f n *) ∗
+      node n In Cn next ∗ own γ_k (◯ prod (keyset _ _ Key In n, dom Cn): keyset_authR Key) ∗
+      own γ_I (◯ In).
 
 
   (*
@@ -51,38 +69,97 @@ Section give_up.
    node n In Cn ∗ own γ_k (◯ prod (keyset _ _ Key In n, Cn): keyset_authR Key) ∗
      own γ_I (◯ In) ∗ ⌜dom In = {[n]}⌝.
  *)
-  
-  Definition globalGhost
-    γ_I γ_f γ_k (r :Node) C (I: @multiset_flowint_ur Key _ _): mpred :=
-    own γ_I (● I) ∗ ⌜globalinv _ _ Key r I⌝ ∗
-      own γ_k (● prod (KS, C): keyset_authR Key) ∗ own (inG0 := nodeset_inG) γ_f (● (dom I)).
 
-  Lemma node_exist_in_tree γ_f n (I: @multiset_flowint_ur Key _ _):
-    inFP γ_f n ∗ own (inG0 := nodeset_inG) γ_f (● (dom I)) ⊢ ⌜n ∈ dom I⌝.
+  Definition own_nodes γ_f (I : @multiset_flowint_ur Key _ _ ) :=
+    ∃ N, ⌜dom N = dom I⌝ ∧ own (inG0 := nodemap_inG) γ_f (● N).
+
+  Definition globalGhost
+    γ_I γ_f γ_k (r :Node) (C : gmap Key data_struct.Value) (I: @multiset_flowint_ur Key _ _): mpred :=
+    own γ_I (● I) ∗ ⌜globalinv _ _ Key r I⌝ ∗
+      own γ_k (● prod (KS, dom C): keyset_authR Key) ∗
+      own_nodes γ_f I
+  (* own (inG0 := nodeset_inG) γ_f (● (dom I)) *).
+
+  Lemma node_exist_in_tree γ_f pn lock n (I: @multiset_flowint_ur Key _ _):
+    inFP γ_f pn lock n ∗ own_nodes γ_f I ⊢ ⌜n ∈ dom I⌝.
   Proof.
     intros; iIntros "(#Hfp & Hown)".
     iDestruct "Hfp" as (n1) "[Hown1 %H1]".
-    iDestruct (own_valid_2 with "Hown Hown1") as %Hown.
+    Check own_valid_2.
+    unfold own_nodes.
+    iDestruct "Hown" as (N0) "(%Hdom & Hown)".
+    iDestruct (own_valid_2 γ_f (● N0: gmap_authR _ _) (◯ (to_agree <$> n1)) with "[$] [$]") as "Hown".
+    iDestruct "Hown" as %Hown.
     rewrite auth_both_valid_discrete in Hown.
-    set_solver.
-  Qed.
+    destruct Hown.
+    Search included gmap.
+    rewrite lookup_included in H2.
+    specialize (H2 n).
+    Search lookup fmap.
+    rewrite lookup_fmap in H2.
+    rewrite H1 in H2.
+    iPureIntro.
+    simpl in H2.
+    Search dom lookup.
+    rewrite <- Hdom.
+    Search dom lookup.
+    unfold dom in *.
+    simpl in *.
+    hnf in N0.
+    rewrite elem_of_dom.
+    Search included Some.
+    apply Some_included_is_Some in H2.
+    auto.
+ Qed.
 
-  Lemma node_conflict_local γ_f γ_k n (rg rg': (number * number)) I_n I_n' C C':
-  node_rep γ_f γ_k n rg I_n C ∗ node_rep γ_f γ_k n rg' I_n' C' -∗ False.
+  Lemma in_node_equiv γ_f p1 p2 lk1 lk2 n:
+    inFP γ_f p1 lk1 n ∗ inFP γ_f p2 lk2 n -∗ ⌜ p1 = p2 /\ lk1 = lk2 ⌝ .
   Proof.
-    iIntros "((((_ & _) & _) & (H1 & _))  & (((_ & _) & _) & (H2 & _)))".
+    iIntros "(H1 & H2)".
+    unfold inFP.
+    iDestruct "H1" as (N1) "(H1 & %K1)".
+    iDestruct "H2" as (N2) "(H2 & %K2)".
+    Search op to_agree.
+    Check own_valid_2.
+    Check own_op.
+    iDestruct (own_valid_2 γ_f (◯ (to_agree <$> N1): gmap_authR Node _) (◯ (to_agree <$> N2): gmap_authR Node _) with "[$H1] [$H2]") as "%Hown".
+    Search valid auth_frag.
+    rewrite auth_frag_op_valid in Hown.
+    Search valid gmap.
+    eapply lookup_valid_Some in Hown; last first.
+    Search lookup op.
+    rewrite lookup_op.
+    Search lookup fmap.
+    rewrite ! lookup_fmap.
+    erewrite K1.
+    rewrite K2.
+    rewrite -  Some_op.
+    auto.
+    apply to_agree_op_inv_L in Hown.
+    iPureIntro.
+    inversion Hown; subst.
+    auto.
+  Qed.
+    
+  Lemma node_conflict_local γ_I γ_k pn lock n I_n I_n' C C':
+  node_rep γ_I γ_k pn lock n I_n C ∗ node_rep γ_I γ_k pn lock n I_n' C' -∗ False.
+  Proof.
+    iIntros "(H1 & H2)".
+    iDestruct "H1" as (rg next) "(_ & (H1 & _))".
+    iDestruct "H2" as (rg' next') "(_ & (H2 & _))".
     iPoseProof (field_at_conflict Ews t_struct_node (DOT _t) with "[$H1 $H2 //]") as "HF"; try done; auto.
   Qed.
 
-  Lemma ghost_snapshot_fp γ_f (Ns: gset Node) n:
-    own (inG0 := nodeset_inG) γ_f (● Ns) ∧ ⌜n ∈ Ns⌝ ==∗
-         own γ_f (inG0 := nodeset_inG) (● Ns) ∗ inFP γ_f n.
+  Lemma ghost_snapshot_fp γ_f (Ns: gmap Node (val * val)) pn lock n:
+    own (inG0 := nodemap_inG) γ_f (● (to_agree <$> Ns)) ∧ ⌜Ns !! n = Some (pn, lock)⌝ ==∗
+         own γ_f (inG0 := nodemap_inG) (● (to_agree <$> Ns)) ∗ inFP γ_f pn lock n.
   Proof.
     iIntros "(H1 & %H2)".
-    iMod (own_update (i:= nodeset_inG) γ_f (● Ns) (● Ns ⋅ ◯ Ns) with "[$]") as "H".
+    iMod (own_update (i:= nodemap_inG) γ_f (● (to_agree <$> Ns)) (● (to_agree <$> Ns) ⋅ ◯ (to_agree <$> Ns)) with "[$]") as "H".
     { apply auth_update_dfrac_alloc. apply _. auto. }
     iDestruct "H" as "(Haa & Haf)".
     iModIntro.
+    unfold inFP.
     by iFrame.
   Qed.
 
@@ -90,37 +167,44 @@ Section give_up.
     ∃ lsh, ⌜field_compatible t_struct_node nil p /\ readable_share lsh⌝ ∧
              (field_at lsh t_struct_node [StructField _lock] lock p ∗ inv_for_lock lock R).
 
-  Definition node_lock_inv_pred γ_f γ_g γ_k node rg I_n C :=
-    my_half γ_g 1 (to_agree node) ∗ node_rep γ_f γ_k node rg I_n C.
+  Definition node_lock_inv_pred γ_I γ_k γ_g pn lock (node : Node) (In : @multiset_flowint_ur Key _ _ ) Cn :=
+    my_half γ_g 1 (to_agree (pn, (lock, (node, (In, Cn))))) ∗ node_rep γ_I γ_k pn lock node In Cn.
   
-  Lemma node_lock_inv_pred_exclusive γ_f γ_g γ_k node rg I_n C:
-      exclusive_mpred (node_lock_inv_pred γ_f γ_g γ_k node rg I_n C).
+  Lemma node_lock_inv_pred_exclusive γ_I γ_k γ_g pn lock node I_n C:
+      exclusive_mpred (node_lock_inv_pred γ_I γ_g γ_k pn lock node I_n C).
   Proof.
     iIntros "((_ & H) & (_ & H'))".
     iPoseProof (node_conflict_local with "[$H $H']") as "?"; done.
   Qed.
 
-  Definition nodeFull γ_f γ_g γ_k n rg : mpred :=
-        ∃ In C, ltree (pointer_of n) (lock_of n) (node_lock_inv_pred γ_f γ_g γ_k n rg In C).
+  (*
+  Definition nodeFull γ_I γ_k γ_g pn lock node : mpred :=
+        ∃ In C, ltree pn lock (node_lock_inv_pred γ_I γ_k γ_g pn lock node In C).
 
-  Definition CSSi γ_I γ_f γ_g γ_k r C I rg: mpred :=
+  
+  Definition CSSi γ_I γ_f γ_k γ_g r C I : mpred :=
                     globalGhost γ_I γ_f γ_k r C I 
-                  ∗ ([∗ set] n ∈ (dom I), public_half γ_g (to_agree n) ∗ nodeFull γ_I γ_g γ_k n rg).
+                  ∗ ([∗ set] n ∈ (dom I), public_half γ_g (to_agree n ∗ nodeFull γ_I γ_k γ_g pn lock n).
+ *)
 
-  Definition CSS γ_I γ_f γ_g γ_k r C rg : mpred := ∃ I, CSSi γ_I γ_f γ_g γ_k r C I rg.
+  Definition CSSi γ_I γ_f γ_k γ_g r C I : mpred := globalGhost γ_I γ_f γ_k r C I
+                  ∗ ([∗ set] n ∈ (dom I), ∃ pn lock In Cn,
+                      public_half γ_g (to_agree (pn, (lock, (n, (In, Cn))))) ∗
+                                  inFP γ_f pn lock n ∗
+                        ltree pn lock (node_lock_inv_pred γ_I γ_k γ_g pn lock n In Cn)).
+                     
+  Definition CSS γ_I γ_f γ_k γ_g r C: mpred := ∃ I, CSSi γ_I γ_f γ_k γ_g r C I.
 
-  Check CSSi.
-
-  Lemma inFP_domm γ_I γ_f γ_g γ_k r C I n rg :
-    inFP γ_f n -∗ CSSi γ_I γ_f γ_g γ_k r C I rg -∗ ⌜n ∈ dom I⌝.
+  Lemma inFP_domm γ_I γ_f γ_k γ_g r C I pn lock n :
+    inFP γ_f pn lock n -∗ CSSi γ_I γ_f γ_k γ_g r C I -∗ ⌜n ∈ dom I⌝.
   Proof.
     iIntros "#Hfp Hcss".
     iDestruct "Hcss" as "((HI & Hglob & Hks & Hdom) & Hbigstar)".
     iPoseProof (node_exist_in_tree with "[$Hfp Hdom]") as "H"; done.
   Qed.
 
-  Lemma int_domm γ_I γ_f γ_g γ_k r C I n In rg :
-    own γ_I (◯ In) -∗ ⌜dom In = {[n]}⌝ -∗ CSSi γ_I γ_f γ_g γ_k r C I rg -∗ ⌜n ∈ dom I⌝.
+  Lemma int_domm γ_I γ_f γ_k γ_g r C I n In :
+    own γ_I (◯ In) -∗ ⌜dom In = {[n]}⌝ -∗ CSSi γ_I γ_f γ_k γ_g r C I -∗ ⌜n ∈ dom I⌝.
   Proof.
     iIntros "Hi Dom_In Hcss".
     iDestruct "Dom_In" as %Dom_In.
@@ -133,27 +217,52 @@ Section give_up.
     set_solver.
   Qed.
 
+  
   (* root is in footprint *)
-  Lemma ghost_update_root γ_I γ_f γ_g γ_k r C rg :
-    CSS γ_I γ_f γ_g γ_k r C rg ==∗
-       CSS γ_I γ_f γ_g γ_k r C rg ∗ inFP γ_f r.
+  Lemma ghost_update_root γ_I γ_f γ_k γ_g r C :
+    CSS γ_I γ_f γ_k γ_g r C ==∗
+       ∃ pr lockr,  CSS γ_I γ_f γ_k γ_g r C ∗ inFP γ_f pr lockr r.
   Proof.
     iIntros "Hcss".
     iDestruct "Hcss" as (I) "((HI & #Hglob & Hks & Hdom) & Hbigstar)".
     iDestruct "Hglob" as %Hglob.
     specialize ((globalinv_root_fp I r) Hglob); intros.
-    iMod (ghost_snapshot_fp γ_f (dom I) r with "[$Hdom //]") as "(Hdom & #Hinfp)".
-    iIntros "!>".
-    iFrame "Hinfp ∗ %".
+    unfold own_nodes.
+    rewrite (big_sepS_elem_of_acc _ (dom I) r); last first. auto.
+    iDestruct "Hdom" as (N1) "(%Hdom & Hdom1)".
+    iDestruct "Hbigstar" as "(Hbigstar & Hb1)".
+    iDestruct "Hbigstar" as (pr lockr Inr Cnr) "(K1 & (#K2 & K3))".
+    iModIntro.
+    iExists _, _. iFrame "K2".
+    iAssert ((∃ (pn lock : valC) (In0 : multiset_flowint_ur) (Cn : gmapO Key valC),
+                  public_half γ_g (to_agree (pn, (lock, (r, (In0, Cn))))) ∗ 
+                  inFP γ_f pn lock r ∗ ltree pn lock (node_lock_inv_pred γ_I γ_k γ_g pn lock r In0 Cn))  )  with "[K1 K3]" as "Hb"; auto.
+    {
+      iExists _, _, _, _. iFrame. iFrame "K2".
+    }
+    iSpecialize ("Hb1" with "Hb").
+    iFrame.
+    iPureIntro. done.
   Qed.
 
+  
   Lemma lock_join lsh1 lsh2 pn lock_in :
-    ⌜readable_share lsh1 /\ readable_share lsh2⌝ ∧ field_at lsh1 t_struct_node (DOT _lock) lock_in pn ∗ field_at lsh2 t_struct_node (DOT _lock) lock_in pn -∗
+    ⌜readable_share lsh1 /\ readable_share lsh2⌝ ∧
+      field_at lsh1 t_struct_node (DOT _lock) lock_in pn ∗
+        field_at lsh2 t_struct_node (DOT _lock) lock_in pn -∗
         ∃ (lsh : share), ⌜readable_share lsh⌝ ∧ field_at lsh t_struct_node (DOT _lock) lock_in pn.
-    Admitted.
+  Proof.
+    iIntros "((%Hrs1 & %Hrs2) & H)".
+    iPoseProof (field_at_share_joins lsh1 lsh2 with "[$H]") as "%HJ". done.
+    destruct HJ as (lsh & HJ).
+    rewrite (field_at_share_join lsh1 lsh2 lsh); auto.
+    iExists lsh. iFrame. iPureIntro.
+    pose proof (@join_readable1 lsh1 lsh2 lsh). auto.
+  Qed.
 
   Lemma share_divided lsh pn (lock_in : val):
-    ⌜readable_share lsh⌝ ∧ field_at lsh t_struct_node (DOT _lock) lock_in pn -∗
+    ⌜readable_share lsh⌝ ∧
+      field_at lsh t_struct_node (DOT _lock) lock_in pn -∗
     (∃ lsh, ⌜readable_share lsh⌝ ∧ field_at lsh t_struct_node (DOT _lock) lock_in pn) ∗
     (∃ lsh, ⌜readable_share lsh⌝ ∧ field_at lsh t_struct_node (DOT _lock) lock_in pn).
   Proof.
@@ -166,6 +275,136 @@ Section give_up.
     apply cleave_readable1 in H1. 
     apply cleave_readable2 in H1'.
     iSplitL "H11"; iExists _; by iFrame.
+  Qed.
+
+  Lemma inv_lock γ_I γ_k γ_g pn lock n In Cn In1 Cn1 In2 Cn2:
+  node_lock_inv_pred γ_I γ_k γ_g pn lock n In Cn ∗
+    inv_for_lock lock (node_lock_inv_pred γ_I γ_k γ_g pn lock n In1 Cn1) -∗
+      node_lock_inv_pred γ_I γ_k γ_g pn lock n In Cn ∗
+        inv_for_lock lock (node_lock_inv_pred γ_I γ_k γ_g pn lock n In2 Cn2).
+  Proof.
+    iIntros "(Hnode & Hinv)".
+    iDestruct "Hinv" as (b') "(Hatm & Hnode')".
+    destruct b'.
+    - iFrame.
+    - iDestruct "Hnode" as "(_ & Hnode)".
+      iDestruct "Hnode'" as "(_ & Hnode')".
+      by iPoseProof (node_conflict_local _ _ pn lock n In In1 Cn Cn1 with "[$Hnode $Hnode']") as "?".
+  Qed.
+      
+  Lemma in_tree_inv' γ_I γ_f γ_k γ_g r (m: gmap Key data_struct.Value) pn lock n In Cn:
+    inFP γ_f pn lock n ∗ node_lock_inv_pred γ_I γ_k γ_g pn lock n In Cn ∗ CSS γ_I γ_f γ_k γ_g r m -∗
+        (node_lock_inv_pred γ_I γ_k γ_g pn lock n In Cn ∗
+             (inv_for_lock lock (node_lock_inv_pred γ_I γ_k γ_g pn lock n In Cn))) ∗
+                  (inv_for_lock lock (node_lock_inv_pred γ_I γ_k γ_g pn lock n In Cn) -∗
+                         CSS γ_I γ_f γ_k γ_g r m).
+  Proof.
+    iIntros "(#HinFP & (Hnode & HCSS))".
+    iDestruct "HCSS" as (In') "HCSS".
+    iPoseProof (inFP_domm γ_I γ_f γ_k γ_g r m In' pn lock n with "[$HinFP] [$HCSS]") as "%".
+    unfold CSSi.
+    iDestruct "HCSS" as "((Hglob & H3) & H4)".
+    rewrite (big_sepS_elem_of_acc _ (dom In') n); last first. auto.
+    iDestruct "H4" as "(H41 & H42)".
+    iDestruct "H41" as (p1 lk1 In1 Cn1) "(H41 & (#K1 & K2))".
+    unfold ltree.
+    iDestruct "K2" as (lsh1) "(%K1 & (K2 & K3))".
+    iDestruct "Hnode" as "(Hn1 & Hn2)".
+    iPoseProof (public_agree with "[$Hn1 $H41]") as "%Hagree".
+    apply to_agree_inj, leibniz_equiv in Hagree.
+    symmetry in Hagree.
+    inversion Hagree; subst.
+    iAssert (node_lock_inv_pred γ_I γ_k γ_g pn lock n In Cn) with "[$Hn1 $Hn2]" as "Hnode".
+    iSplitL "Hnode K3"; iFrame. 
+    iIntros "H".
+    iAssert (∃ (pn0 lock0 : valC) (In0 : multiset_flowint_ur) (Cn0 : gmapO Key valC),
+             public_half γ_g (to_agree (pn0, (lock0, (n, (In0, Cn0))))) ∗ inFP γ_f pn0 lock0 n ∗
+             ∃ lsh : share,
+               ⌜field_compatible t_struct_node [] pn0 ∧ readable_share lsh⌝
+               ∧ @field_at _ _ _ CompSpecs lsh t_struct_node (DOT _lock) lock0 pn0 ∗
+               inv_for_lock lock0 (node_lock_inv_pred γ_I γ_k γ_g pn0 lock0 n In0 Cn0))
+        with "[$H41 $K2 $H]" as "H1"; auto.
+      iSpecialize ("H42" with "H1").
+      iFrame.
+  Qed.
+  
+  Lemma in_node_inv γ_I γ_f γ_k γ_g r (m: gmap Key data_struct.Value) pn lock n:
+    inFP γ_f pn lock n ∗ CSS γ_I γ_f γ_k γ_g r m -∗
+      (∃ In C, (inv_for_lock lock (node_lock_inv_pred γ_I γ_k γ_g pn lock n In C) ∗
+               (inv_for_lock lock (node_lock_inv_pred γ_I γ_k γ_g pn lock n In C)
+                -∗ CSS γ_I γ_f γ_k γ_g r m))) ∧                                       
+      (∃ R, (ltree pn lock R) ∗
+              (ltree pn lock  R -∗ CSS γ_I γ_f γ_k γ_g r m)).
+
+  Proof.
+    iIntros "(#H1 & H2)".
+    iDestruct "H2" as (I) "H2".
+    iPoseProof (inFP_domm γ_I γ_f γ_k γ_g r m I pn lock n with "[$] [$]") as "%".
+    iDestruct "H2" as "((H2 & H3) & H4)".
+    unfold own_nodes.
+    Check big_sepS_elem_of_acc _ (dom I) n.
+    rewrite (big_sepS_elem_of_acc _ (dom I) n); last first; auto.
+    iDestruct "H4" as "(Hn & Hbigstar)".
+    iDestruct "Hn" as (p lk In C) "(Hp & (#Hn1 & Hn))".
+    iDestruct "Hn" as (lsh) "(%Hn1 & (Hn2 & Hn3))".
+    iPoseProof (in_node_equiv γ_f pn p lock lk n with "[$H1 $Hn1]") as "%K1".
+    destruct K1; subst.
+    iSplit.
+    - iExists _, _.
+      iFrame.
+      iIntros "H".
+      iExists I. iFrame.
+      iAssert ((∃ (pn lock : valC) (In0 : multiset_flowint_ur) (Cn : gmapO Key valC),
+                  public_half γ_g (to_agree (pn, (lock, (n, (In0, Cn))))) ∗ 
+                  inFP γ_f pn lock n ∗ ltree pn lock (node_lock_inv_pred γ_I γ_k γ_g pn lock n In0 Cn))  )  with "[$H $Hn2 $Hp]" as "Hb"; auto.
+      by iSpecialize ("Hbigstar" with "[$Hb]").
+    - unfold ltree.
+      iExists _.
+      iSplitL "Hn2 Hn3".
+      iExists lsh. iSplit. done. iFrame.
+      iIntros "H".
+      iDestruct "H" as (lsh1) "H".
+      iExists I. iFrame.
+      iDestruct "H" as "(%Hm1 & Hm2)".
+      iAssert ((∃ (pn lock : valC) (In0 : multiset_flowint_ur) (Cn : gmapO Key valC),
+                  public_half γ_g (to_agree (pn, (lock, (n, (In0, Cn))))) ∗ 
+                  inFP γ_f pn lock n ∗
+                  ∃ lsh0 : share,
+                    ⌜field_compatible t_struct_node [] pn ∧ readable_share lsh0⌝
+                    ∧ @field_at _ _ _ CompSpecs lsh0 t_struct_node (DOT _lock) lock pn ∗
+                    inv_for_lock lock (node_lock_inv_pred γ_I γ_k γ_g pn lock n In0 Cn)))
+        with "[$Hp $Hm2]" as "Hb"; auto.
+      iSpecialize ("Hbigstar" with "Hb").
+      iFrame.
+  Qed.
+  
+  Lemma lock_alloc (B: Type) (b: _ -> B -> mpred) (Q : B → mpred) γ_I γ_f γ_g γ_k r pn lock n:
+         atomic_shift (λ C, CSS γ_I γ_f γ_g γ_k r C) ⊤ ∅ b Q ∗ inFP γ_f pn lock n -∗
+         |={⊤}=> atomic_shift (λ C, CSS γ_I γ_f γ_g γ_k r C) ⊤ ∅ b Q ∗ inFP γ_f pn lock n ∗
+            (∃ lsh : share,
+      ⌜readable_share lsh⌝ ∧ field_at lsh t_struct_node (DOT _lock) lock pn).
+  Proof.
+    iIntros "(AU & #H)".
+    iMod "AU" as (m) "[Hm HClose]".
+    iPoseProof (in_node_inv γ_I γ_f γ_g γ_k r with "[$H $Hm]") as "InvLock".
+    iDestruct "InvLock" as "(_ & InvLock)".
+    iDestruct "InvLock" as (R) "[H1 H2]".
+    iDestruct "H1" as (lsh) "(%Hfr & (H12 & H13))".
+    destruct Hfr as (Hf & Hr).
+    iPoseProof (share_divided with "[$H12]") as "H1"; auto.
+    iDestruct "H1" as "(H1 & H1')".
+    iDestruct "H1" as (lsh1) "(% & H1)".
+    iDestruct "H1'" as (lsh2) "(% & H1')".
+    iAssert (∃ lsh, ⌜readable_share lsh⌝ ∧ @field_at _ _ _ CompSpecs lsh t_struct_node (DOT _lock) lock pn) with "[$H1]" as "H3". done.
+    iAssert (∃ lsh, ⌜readable_share lsh⌝ ∧ @field_at _ _ _ CompSpecs lsh t_struct_node (DOT _lock) lock pn) with "[$H1']" as "H3'". done.
+    iFrame. iFrame "H".
+    iDestruct "H3" as (lsh') "(% & H3)".
+    iAssert (∃ lsh, ⌜field_compatible t_struct_node [] pn ∧ readable_share lsh ⌝ ∧
+          (@field_at _ _ _ CompSpecs lsh t_struct_node (DOT _lock) lock pn ∗
+           inv_for_lock lock R))  with "[H3 H13]" as "H1".
+    { iExists _. iFrame. done. }
+    iSpecialize ("H2" with "H1").
+    by iSpecialize ("HClose" with "H2").
   Qed.
   
 End give_up.
