list_giveup_specs.v
@@ -1,17 +1,42 @@
 Require Import VST.concurrency.conclib.
+From iris.algebra Require Import excl auth gmap agree gset.
+Require Import flows.inset_flows.
+Require Import flows.auth_ext.
+Require Import flows.multiset_flows.
+Require Import flows.flows.
+Require Import iris_ora.algebra.gmap.
+Require Import iris_ora.logic.own.
+Require Import iris_ora.algebra.ext_order.
+Require Import iris_ora.algebra.frac_auth.
 Require Import VST.floyd.proofauto.
 Require Import VST.atomics.general_locks.
-Require Import bst.list_giveup. (* list_giveup.c *)
-Require Import bst.puretree.
-Require Import bst.data_struct.
-Require Import bst.giveup_lib.
-(* Require Import bst.giveup_specs. *)
-Require Import VST.atomics.verif_lock_atomic.
 Require Import VST.floyd.library.
+Require Import VST.atomics.verif_lock_atomic.
+Require Import tmpl.puretree.
+Require Import tmpl.list_giveup. (* list_giveup.c *)
+Require Import tmpl.keyset_ra_ora.
+Require Import tmpl.puretree.
+Require Import tmpl.data_struct.
+Require Import tmpl.flows_ora.
+
 
 #[export] Instance CompSpecs : compspecs. make_compspecs prog. Defined.
 Definition Vprog : varspecs.  mk_varspecs prog. Defined.
 
+#[global] Instance gmap_inhabited V : Inhabitant (gmap key V).
+Proof. unfold Inhabitant; apply empty. Defined.
+
+#[global] Instance number_inhabited: Inhabitant number.
+Proof. unfold Inhabitant; apply Pos_Infinity. Defined.
+
+Section give_up_traverse.
+  Locate VSTGS0.
+  Context `{N: NodeRep } `{EqDecision K} `{Countable K}.
+  Locate VSTGS0.
+  Context `{!cinvG Σ, atom_impl : !atomic_int_impl (Tstruct _atom_int noattr),
+            !flowintG Σ, !nodesetG Σ, !keysetG Σ, !keymapG Σ, inG Σ (frac_authR (agreeR Node))}.
+  Context (Hsize: node_size = 1%nat).
+  
 Definition struct_dlist := Tstruct _DList noattr.
 Definition t_struct_node := Tstruct _node_t noattr.
 Definition t_struct_nodeds := Tstruct _node noattr.
@@ -29,89 +54,73 @@ Definition fst_thrd_list: list (val * val * val * val) -> list (val * val) :=
 Definition fst_frth_list: list (val * val * val * val) -> list (val * val) :=
   map (fun '(x, _, _, y) => (x, y)).
 
-Section give_up.
-  Context {N: NodeRep}.
-  Context (Hsize: node_size = 1%nat).
-
 Definition surely_malloc_spec :=
   DECLARE _surely_malloc
    WITH t: type, gv: globals
    PRE [ size_t ]
        PROP (and (Z.le 0 (sizeof t)) (Z.lt (sizeof t) Int.max_unsigned);
-             complete_legal_cosu_type t = true; natural_aligned natural_alignment t = true)
+                complete_legal_cosu_type t = true;
+                natural_aligned natural_alignment t = true)
        PARAMS (Vptrofs (Ptrofs.repr (sizeof t))) GLOBALS (gv)
        SEP (mem_mgr gv)
     POST [ tptr tvoid ]
-    EX p: _,
+    ∃ p: _,
        PROP ()
        RETURN (p)
-       SEP (mem_mgr gv; malloc_token Ews t p * data_at_ Ews t p).
+       SEP (mem_mgr gv; malloc_token Ews t p; data_at_ Ews t p).
+
+Fixpoint list_to_gmap_aux (l : list Node) (key : nat) : gmap nat Node :=
+  match l with
+  | [] => ∅
+  | x :: xs => <[key:=x]> (list_to_gmap_aux xs (S key))
+  end.
+
+Definition list_to_gmap (l : list Node) : gmap nat Node :=
+  list_to_gmap_aux l 0.
 
 Definition insertOp_spec :=
   DECLARE _insertOp
-    WITH x: Z, stt: Z, v: val, p: val, l: val, dl: val, next: list val,
-                    g: gname, gv: globals
+    WITH x: Z, v: val, stt: Z, p: Node, tp: val, l: val, dl: val,
+                  Ip : @flowintT _ K_multiset_ccm  _ _,
+                    Cp : (gmap Key data_struct.Value),
+                     (* pnext : gmap nat Node, *)
+                      next: list Node,
+                        gv: globals
   PRE [ tptr (tptr t_struct_nodeds), tint, tptr tvoid, tint, tptr (struct_dlist)]
-  PROP (repable_signed x; is_pointer_or_null v;
+  PROP (repable_signed x; is_pointer_or_null v; (*node_size = length ((gmap_to_node_list pnext)); *)
+        length next = node_size;
+        (* is_pointer_or_null (Znth 0 (gmap_to_node_list pnext)); *)
         is_pointer_or_null (Znth 0 next);
-        length next = node_size)
+        tp = nullval)
   PARAMS (p; Vint (Int.repr x); v; Vint (Int.repr stt); l)
   GLOBALS (gv)
-  SEP (mem_mgr gv; 
-                     field_at Tsh (struct_dlist) [StructField _list] dl l *
-                     (* field_at Ews (struct_dlist) [StructField _size] (Vptrofs (Ptrofs.repr 2%Z)) l * *)
-                     data_at Ews (tarray (tptr tvoid) (Zlength next)) next dl * 
-                     (* (!!(p = r.1.1.1 /\ p = nullval)  && seplog.emp); *)
-       data_at Ews (tptr t_struct_nodeds) nullval p)
+  SEP (mem_mgr gv; node tp Ip Cp (list_to_gmap next);
+       field_at Tsh (struct_dlist) (DOT _list) dl l;
+       data_at Ews (tptr t_struct_nodeds) tp p;
+                   (* field_at Ews (struct_dlist) [StructField _size] (Vptrofs (Ptrofs.repr 2%Z)) l ∗ *)
+                   (* data_at Ews (tarray (tptr tvoid) (Zlength (gmap_to_node_list pnext) )) (gmap_to_node_list pnext) dl *)
+       data_at Ews (tarray (tptr tvoid) (Zlength next)) next dl
+       )
   POST[ tvoid ]
-  EX (pnt : val),
+  ∃ (pnt : Node),
   PROP (pnt <> nullval)
   LOCAL ()
-  SEP (mem_mgr gv; data_at Ews (tptr t_struct_nodeds) pnt p;
-       node_rep_R pnt (Some (Some (x, v, next))) g;
+  SEP (mem_mgr gv; node pnt Ip Cp (list_to_gmap next); node tp Ip Cp (list_to_gmap next);
        field_at Tsh struct_dlist (DOT _list) dl l;
-       data_at Ews (tarray (tptr tvoid) (Zlength next)) next dl).
+       data_at Ews (tptr t_struct_nodeds) pnt p;
+       (*data_at Ews (tarray (tptr tvoid) (Zlength (gmap_to_node_list pnext))) (gmap_to_node_list pnext) dl*)
+     data_at Ews (tarray (tptr tvoid) (Zlength next)) next dl  
 
+  ).
 
-Definition post_insert_giveup1 (p pnt : val) (x: Z) v
-  min max (trl : list (val * val * val * val)) (ptl : list val) g :=
-       iter_sepcon (fun pn => malloc_token Ews t_struct_node pn) (fst_list trl) * 
-       iter_sepcon (fun pn => field_at Ews t_struct_node (DOT _t) (Vlong (Int64.repr 0)) pn)
-         (fst_list trl) * 
-       iter_sepcon (fun lk => atomic_int_at Ews (vint 0) lk) (snd_list trl) * 
-       iter_sepcon (fun fs => field_at Ews t_struct_node (DOT _lock) (snd fs) (fst fs))
-         (fst_snd_list trl) * 
-       iter_sepcon (fun ft => field_at Ews t_struct_node (DOT _min) (snd ft) (fst ft))
-         (fst_thrd_list trl) * 
-       iter_sepcon (fun ff => field_at Ews t_struct_node (DOT _max) (snd ff) (fst ff))
-         (fst_frth_list trl) *
-       iter_sepcon(fun ptl => node_rep_R ptl (Some (@None ghost_info)) g) ptl *
-       node_rep_R pnt (Some (Some (x, v, (fst_list trl)))) g *
-       field_at Ews t_struct_node (DOT _t) pnt p *
-       field_at Ews t_struct_node (DOT _min) (vint min) p * 
-       field_at Ews t_struct_node (DOT _max) (vint max) p.
-
-Definition post_insert_giveup2 (p pnt: val) (x: Z) v 
-  min max (trl : list (val * val * val * val)) (ptl : list val) (r: node_info) g :=
-       iter_sepcon (fun pn => malloc_token Ews t_struct_node pn) (fst_list trl) * 
-       iter_sepcon (fun '(tp, pn) => field_at Ews t_struct_node (DOT _t) tp pn)
-         (combine ptl (fst_list trl)) * 
-       iter_sepcon (fun lk => atomic_int_at Ews (vint 0) lk) (snd_list trl) * 
-       iter_sepcon (fun fs => field_at Ews t_struct_node (DOT _lock) (snd fs) (fst fs))
-         (fst_snd_list trl) * 
-       iter_sepcon (fun ft => field_at Ews t_struct_node (DOT _min) (snd ft) (fst ft))
-         (fst_thrd_list trl) * 
-       iter_sepcon (fun ff => field_at Ews t_struct_node (DOT _max) (snd ff) (fst ff))
-         (fst_frth_list trl) *
-       iter_sepcon(fun ptl => node_rep_R ptl r.2 g) ptl *
-       node_rep_R pnt (Some (Some (x, v, (fst_list trl)))) g *
-       field_at Ews t_struct_node (DOT _t) pnt p * 
-       field_at Ews t_struct_node (DOT _min) (vint min) p * 
-       field_at Ews t_struct_node (DOT _max) (vint max) p.
 
 Definition insertOp_giveup_spec :=
   DECLARE _insertOp_giveup
-    WITH x: Z, stt: Z,  v: val, p: val, tp: val, min: Z, max: Z, r: node_info, g: gname, gv: globals
+    WITH x: Z, v: val, stt: Z, p: Node, tp: val, min: Z, max: Z,
+                  Ip : @flowintT _ K_multiset_ccm  _ _,
+                    Cp : (gmap Key data_struct.Value),
+                      next : list Node,
+                        sh: share, gv: globals
   PRE [ tptr t_struct_node, tint, tptr tvoid, tint ]
   PROP (repable_signed min; repable_signed max; repable_signed x;
         is_pointer_or_null v; is_pointer_or_null v; is_pointer_or_null tp)
@@ -119,60 +128,27 @@ Definition insertOp_giveup_spec :=
   GLOBALS (gv)
   SEP (mem_mgr gv;
        match (Int.eq (Int.repr stt) (Int.repr 2%Z)) with
-        | true => (!!(tp = nullval /\ (r.2 = Some None) ) && seplog.emp)
-        | false => (!!(tp <> nullval) && seplog.emp)
+        | true => ⌜tp = nullval⌝ ∧ emp
+        | false => ⌜tp <> nullval⌝ ∧ emp 
        end;
        field_at Ews t_struct_node (DOT _t) tp p;
        field_at Ews t_struct_node (DOT _min) (vint min) p;
        field_at Ews t_struct_node (DOT _max) (vint max) p;
-       node_rep_R tp r.2 g )
+       node tp Ip Cp (list_to_gmap next))
   POST[ tvoid ] (* triple (pointer, lock, min, max) *)
-  EX (pnt : val) (trl : list (val * val * val * val)) (ptl : list val),
+  ∃ (pnt : val) (trl : list (val * val * val * val)) (ptl : list val),
   PROP (pnt <> nullval)
   LOCAL ()
   SEP (mem_mgr gv;
        (match (Int.eq (Int.repr stt) (Int.repr 2%Z)) with
-        | true => (post_insert_giveup1 p pnt x v min max trl ptl g)
-        | _    => (post_insert_giveup2 p pnt x v min
-                   max trl ptl r g)
+        | true => ⌜tp = nullval⌝ ∧ emp
+        | _    =>  ⌜tp <> nullval⌝ ∧ emp 
         end)).
 
 Definition Gprog : funspecs :=
     ltac:(with_library prog [acquire_spec; release_spec; makelock_spec;  
                              insertOp_giveup_spec; insertOp_spec;
                              surely_malloc_spec ]).
-
-Check iter_sepcon.
-Lemma test (trl : list (val * val * val * val)):
-  (iter_sepcon (fun '(pn, lk, fs, ft) =>
-                  malloc_token Ews t_struct_node pn *
-                  field_at Ews t_struct_node (DOT _t) (Vlong (Int64.repr 0)) pn *
-                  atomic_int_at Ews (vint 0) lk *
-                  field_at Ews t_struct_node (DOT _lock) lk pn *
-                  field_at Ews t_struct_node (DOT _min) fs pn *
-                  field_at Ews t_struct_node (DOT _max) ft pn) trl ) |--
-iter_sepcon (fun pn => malloc_token Ews t_struct_node pn) (fst_list trl) *
-       iter_sepcon (fun pn => field_at Ews t_struct_node (DOT _t) (Vlong (Int64.repr 0)) pn)
-         (fst_list trl) *
-       iter_sepcon (fun lk => atomic_int_at Ews (vint 0) lk) (snd_list trl) * 
-       iter_sepcon (fun fs => field_at Ews t_struct_node (DOT _lock) (snd fs) (fst fs))
-         (fst_snd_list trl) *
-       iter_sepcon (fun ft => field_at Ews t_struct_node (DOT _min) (snd ft) (fst ft))
-         (fst_thrd_list trl) *
-       iter_sepcon (fun ff => field_at Ews t_struct_node (DOT _max) (snd ff) (fst ff))
-         (fst_frth_list trl).
-Proof.
-  simpl.
-  Search iter_sepcon.
-  induction trl. simpl.
-  cancel.
-  replace (a :: trl) with ([a]++trl); auto.
-  rewrite ! iter_sepcon_app.
-  sep_apply IHtrl.
-  simpl.
-  destruct a.
-  destruct p. destruct p. simpl. entailer !.
-Qed.
 
 Lemma insertOp_bst: semax_body Vprog Gprog f_insertOp_giveup insertOp_giveup_spec.
 Proof.
@@ -192,47 +168,76 @@ Proof.
   forward.
   forward.
   forward_call release_nonatomic (lock).
-  forward_if(PROP (field_compatible t_struct_node (DOT _t) p)
-     LOCAL (temp _t'20 p1; temp _t'19 lst; temp _l lock; temp _t'21 lst; temp _t'2 p1; temp _t'1 lst;
+  forward_if(PROP ( )
+     LOCAL (temp _t'20 (Znth 0 (upd_Znth 0 (default_val (tarray (tptr tvoid) 1)) p1)); 
+     temp _t'19 lst; temp _l lock; temp _t'21 lst; temp _t'2 p1; temp _t'1 lst;
      temp _t'22 (Vlong (Int64.repr (Int.signed (Int.repr 1))));
      lvar _dlist (Tstruct _DList noattr) v_dlist; gvars gv; temp _p p; temp _x (vint x); 
      temp _value v; temp _status (vint stt))
-     SEP ((match (Int.eq (Int.repr stt) (Int.repr 2%Z)) with
-           | true => (EX (pnt : val),
-                      (!!(pnt <> nullval) && seplog.emp) *
-                        iter_sepcon(fun ptl => node_rep_R ptl (Some (@None ghost_info)) g) [nullval] *
-                        node_rep_R pnt (Some (Some (x, v, [p1]))) g * data_at Ews (tptr t_struct_nodeds) pnt (field_address t_struct_node (DOT _t) p) * data_at Ews t_struct_node (nullval , (lock, (vint x, vint Int.max_signed))) p1)
-           | false =>  (EX (pnt: val), (!!(pnt <> nullval) && seplog.emp) *
-                                        iter_sepcon(fun ptl => node_rep_R ptl r.2 g) [tp] * 
-                                      node_rep_R pnt (Some (Some (x, v, [p1]))) g * data_at Ews (tptr t_struct_nodeds) pnt (field_address t_struct_node (DOT _t) p) * data_at Ews t_struct_node (tp, (lock, (vint x, vint max))) p1)
-           end); atomic_int_at Ews (vint 0) lock; mem_mgr gv; malloc_token Ews t_struct_node p1;
-     malloc_token Ews (tarray (tptr tvoid) 1) lst;
-     data_at Ews (tarray (tptr tvoid) 1) [p1] lst;
+     SEP (atomic_int_at Ews (vint 0) lock; mem_mgr gv; malloc_token Ews t_struct_node p1;
+     data_at Ews t_struct_node ((default_val t_struct_node).1, (lock, (default_val t_struct_node).2.2))
+       p1; malloc_token Ews (tarray (tptr tvoid) 1) lst;
+     data_at Ews (tarray (tptr tvoid) 1) (upd_Znth 0 (default_val (tarray (tptr tvoid) 1)) p1) lst;
      data_at Tsh (Tstruct _DList noattr) (lst, Vlong (Int64.repr (Int.signed (Int.repr 1)))) v_dlist;
-     field_at Ews t_struct_node (DOT _min) (vint min) p;
-     field_at Ews t_struct_node (DOT _max) (vint max) p)).
-  - rewrite H5; simpl.
+     if Int.eq (Int.repr stt) (Int.repr 2) then ⌜tp = nullval⌝ ∧ emp else ⌜tp ≠ nullval⌝ ∧ emp;
+     field_at Ews t_struct_node (DOT _t) tp p; field_at Ews t_struct_node (DOT _min) (vint min) p;
+     field_at Ews t_struct_node (DOT _max) (vint max) p; node tp Ip Cp (list_to_gmap [p1]))).
+  - rewrite H7; simpl.
     Intros.
     forward. forward. forward.
-    assert_PROP (field_compatible t_struct_node [] p1) by entailer!.
+    assert_PROP(field_compatible t_struct_node [] p1) by entailer!.
     assert_PROP(field_compatible t_struct_node (DOT _t) p) by entailer !.
     assert (field_address t_struct_node (DOT _t) p  = p) as I.
     rewrite ->  field_compatible_field_address, isptr_offset_val_zero; auto.
+    
     (* call insertOp *)
-
-    forward_call(x, stt, v, (field_address t_struct_node [StructField _t] p), v_dlist, lst, [p1] ,
-                  g, gv).
+    forward_call(x, v, stt, (field_address t_struct_node [StructField _t] p), tp, v_dlist, lst, Ip, Cp, [p1] , gv).
     {
+      subst tp.
       entailer !. simpl.
-      change ((((0 + Z.pos (8 * 8) - 1) `div` Z.pos (8 * 8) * Z.pos (8 * 8)) `div` 8)) with 0.
-      rewrite I isptr_offset_val_zero; auto.
-      replace (vint stt) with (vint 2); f_equal; auto.
+      rewrite I. rewrite isptr_offset_val_zero.
+      replace (vint stt) with (vint 2); f_equal; auto. auto.
     }
     unfold_data_at (data_at _ _ _ v_dlist).
     cancel.
-    entailer !. 
+    entailer !.
+    assert (list_to_gmap next = list_to_gmap [p1]). admit.
+    rewrite H8.
+    entailer !.
     Intros pnt.
-    forward. forward. entailer !. list_solve.
+    admit.
+
+
+  - rewrite Int.eq_false; auto.
+    Intros.
+    forward. forward. forward. forward.
+    forward. forward. forward. forward.
+    forward. forward. forward. forward.
+    assert_PROP (field_compatible t_struct_node [] p1) by entailer!.
+    (* call insertOp *)
+    assert_PROP(field_compatible t_struct_node (DOT _t) p) by entailer !.
+    assert (field_address t_struct_node (DOT _t) p  = p) as I.
+    rewrite -> field_compatible_field_address, isptr_offset_val_zero; auto.
+    (* call insertOp *)
+    forward_call(x, v, stt, (field_address t_struct_node [StructField _t] p), nullval, v_dlist, lst, Ip, Cp, [p1] , gv).
+    unfold_data_at (data_at _ _ _ v_dlist).
+    entailer !.
+    change (Vlong (Int64.repr 0)) with nullval.
+    assert (list_to_gmap next = list_to_gmap [p1]). admit.
+    rewrite H23.
+    cancel.
+    unfold_data_at (data_at _ _ _ v_dlist).
+    
+    
+    {
+      subst tp.
+      entailer !. simpl.
+      rewrite I. rewrite isptr_offset_val_zero.
+      replace (vint stt) with (vint 2); f_equal; auto. auto.
+    }
+
+    
+    forward. forward. forward. forward. forward. forward. entailer !. list_solve.
     forward. forward. forward. entailer !. list_solve.
     forward.
     rewrite H5.
