list_inst.v
@@ -1,118 +1,172 @@
 Require Import VST.concurrency.conclib.
+From iris.algebra Require Import excl auth gmap agree gset.
+Require Import flows.inset_flows.
+Require Import flows.auth_ext.
+Require Import flows.multiset_flows.
+Require Import flows.flows.
+Require Import iris_ora.algebra.gmap.
+Require Import iris_ora.logic.own.
+Require Import iris_ora.algebra.ext_order.
+Require Import iris_ora.algebra.frac_auth.
 Require Import VST.floyd.proofauto.
 Require Import VST.atomics.general_locks.
-Require Import Coq.Sets.Ensembles.
-Require Import bst.puretree.
-Require Import bst.list.
-Require Import bst.data_struct.
-Require Import VST.atomics.verif_lock_atomic.
 Require Import VST.floyd.library.
+Require Import VST.atomics.verif_lock_atomic.
+Require Import tmpl.puretree.
+Require Import tmpl.list. (*binary search tree*)
+Require Import tmpl.keyset_ra_ora.
+Require Import tmpl.puretree.
+Require Import tmpl.data_struct.
+Require Import tmpl.flows_ora.
+
 
 #[export] Instance CompSpecs : compspecs. make_compspecs prog. Defined.
 Definition Vprog : varspecs.  mk_varspecs prog. Defined.
+
+#[global] Instance gmap_inhabited V : Inhabitant (gmap key V).
+Proof. unfold Inhabitant; apply empty. Defined.
+
+#[global] Instance number_inhabited: Inhabitant number.
+Proof. unfold Inhabitant; apply Pos_Infinity. Defined.
+
+Section give_up_traverse.
+  Locate VSTGS0.
+  Context `{N: NodeRep } `{EqDecision K} `{Countable K}.
+  Locate VSTGS0.
+  Context `{!cinvG Σ, atom_impl : !atomic_int_impl (Tstruct _atom_int noattr),
+            !flowintG Σ, !nodesetG Σ, !keysetG Σ, !keymapG Σ, inG Σ (frac_authR (agreeR Node))}.
+  
 
 (* struct node {int key; void *value; struct tree_t *left, *right;} node;*)
 Definition t_struct_list := Tstruct _node noattr.
 (* Define for dynamic list *)
 Definition struct_dlist := Tstruct _DList noattr.
 
-#[local] Obligation Tactic := idtac.
-(* node_rep_R r.1.1.1 r.1.2 r.2 g, and r is type of node_info *)
-#[local] Program Instance my_specific_tree_rep : NodeRep := {
-    node_rep_R := fun (tp : val) (g_info : option (option ghost_info)) g =>
-      if eq_dec tp nullval
-      then !!(g_info = Some None) && seplog.emp
-      else (EX (x : Z), EX (v next : val),
-      !!(g_info = Some (Some (x, v, [next])) /\ and (Z.le Int.min_signed x) (Z.le x Int.max_signed) /\
-       is_pointer_or_null next /\ (tc_val (tptr Tvoid) v)) &&
-       data_at Ews t_struct_list ((Vint (Int.repr x)), (v, next)) tp *
-       malloc_token Ews t_struct_list tp); node_size := 1 }.
-Next Obligation.
-  simpl.
-  intros tp g_info g.
-  destruct (EqDec_val tp nullval); [ | Intros x v next]; entailer !.
-Defined.
-Next Obligation.
-  simpl.
-  intros tp g_info g.
-  destruct (EqDec_val tp nullval); [ | Intros x v next]; entailer !.
-Defined.
-Next Obligation.
-  by intros g_info.
-Defined.
-    
-Definition extract_node_pn (node: node_info) : list val :=
-  match node.2 with
-  | Some (Some (_, _, lst)) => lst
-  | _ => []
-  end.
+(* struct tree_t {node *t; lock_t *lock; int min; int max; } tree_t; *)
+(* Definition t_struct_tree_t := Tstruct _tree_t noattr. *)
 
-(* Spec of findnext function *)
-(* FOUND = 0, NOTFOUND = 1, NULLNEXT = 2 (NULLNEXT = NULL || NEXT ) *)
+(* node_rep_R r.1.1.1 r.1.2 r.2 g, and r is type of node_info *)
+
+(*
+Class NodeRep : Type := {
+    node : val → @multiset_flowint_ur Key _ _ → gmap Key Value -> gmap nat Node -> mpred;
+    (* node_sep_star: ∀ n I_n I_n' C C', node n I_n C ∗ node n I_n' C' -∗ False; *)
+    node_rep_R_valid_pointer: forall n I_n C next, node n I_n C next -∗ valid_pointer n;
+    node_rep_R_pointer_null: forall n I_n C next, node n I_n C next -∗ ⌜is_pointer_or_null n⌝;
+    node_size: nat;
+}.
+
+ *)
+
+#[local] Obligation Tactic := idtac.
+
+#[local] Program Instance my_specific_tree_rep : NodeRep := {
+  node := fun (n : Node) (In : @multiset_flowint_ur Key _ _) (C: gmap Key data_struct.Value)
+            (next:  gmap nat Node) =>
+  if eq_dec n nullval
+  then ⌜∀ y : Key, ¬ in_outsets val_EqDecision Node_countable Key y In ∧
+                     ¬ ∃ n1 : Node, n1 ≠ n ∧ in_inset val_EqDecision Node_countable Key y In n1 ∧
+                     C = ∅⌝ ∧ emp
+  else
+  (∃ (x : Z) (v : val),
+      ⌜and (Z.le Int.min_signed x) (Z.le x Int.max_signed) /\
+       is_pointer_or_null (next !!! 0)  /\
+          (tc_val (tptr Tvoid) v) ∧ C = {[x := v]} ∧
+        (forall y, in_outset _ _ _ y In (next !!! 0) <-> Z.lt x y ∧ in_inset _ _ _ y In n) ∧
+        (forall y, in_outsets _ _ _ y In -> in_outset _ _ _ y In (next !!! 0)) ⌝ ∧
+       data_at Ews t_struct_list (Vint (Int.repr x), (v, (next !!! 0))) n ∗
+       malloc_token Ews t_struct_list n); node_size := 1}.
+(* ; node_rep_R_valid_pointer }. *)
+Next Obligation.
+  intros n In Cn next. 
+  destruct (EqDec_val n nullval). 
+  - simpl. rewrite e. auto.
+  - rewrite if_false; auto. iIntros "H".
+    iDestruct "H" as (x v) "(%HJ & (H1 & H2))".
+    iStopProof. entailer !.
+Defined.
+Next Obligation.
+  intros n In Cn next.
+  destruct (EqDec_val n nullval).
+  - simpl. rewrite e. auto.
+  - rewrite if_false; auto.
+    iIntros "H".
+    iDestruct "H" as (x v) "(%HJ & (H1 & H2))".
+    iStopProof. entailer !.
+Defined.
 
 (* Spec of findnext function *)
 (* FOUND = 0, NOTFOUND = 1, NULLNEXT = 2 (NULLNEXT = NULL || NEXT ) *)
 Definition findnext_spec :=
   DECLARE _findNext
-  WITH x: Z, p: val, n: val, n_pt : val, r: node_info,
-                g: gname, sh: share, gv: globals
+  WITH x: Z, p: Node, n: val, n_pt : val, Ip : flowintT,
+                Cp : (gmap Key data_struct.Value), nextp : gmap nat Node, sh: share, gv: globals
   PRE [ tptr t_struct_list, tptr (tptr tvoid), tint ]
-          PROP (writable_share sh(*; is_pointer_or_null pa; is_pointer_or_null pb*) )
+          PROP (writable_share sh;
+                (Int.min_signed ≤ x ≤ Int.max_signed)%Z
+          (*; is_pointer_or_null pa; is_pointer_or_null pb*) )
           PARAMS (p; n; Vint (Int.repr x)) GLOBALS (gv)
-          SEP (node_rep_R r.1.1.1 r.2 g * (!!(p = r.1.1.1 /\ p <> nullval) && seplog.emp) *
+          SEP (node p Ip Cp nextp ∗ ⌜p <> nullval /\ in_inset _ _ _ x Ip p⌝ ∧
                (* field_at sh (t_struct_tree) [StructField _t] r.1.1.1 p; *)
                data_at sh (tptr tvoid) n_pt n)
   POST [ tint ]
-  EX (stt: enum), EX (n' next : val),
+  ∃ (stt: enum), ∃ (n' next : Node),
          PROP (match stt with
                | F | NF => (n' = p)
                | NN => (n' = next)
                end)
         LOCAL (temp ret_temp (enums stt))
         SEP (match stt with
-               | F | NF => data_at sh (tptr tvoid) n_pt n
-               | NN => !!(n' ∈ extract_node_pn r) && data_at sh (tptr tvoid) next n
-             end *
-               node_rep_R r.1.1.1 r.2 g) .
+               | F | NF => ⌜¬in_outsets _ _ _ x Ip⌝ ∧ data_at sh (tptr tvoid) n_pt n
+               | NN => ⌜in_outset _ _ _ x Ip next⌝ ∧ data_at sh (tptr tvoid) next n
+             end ∗
+               node p Ip Cp nextp).
 
 Lemma findNext: semax_body Vprog Gprog f_findNext findnext_spec.
 Proof.
   start_function.
-  unfold node_rep_R.
-  unfold my_specific_tree_rep.
   Intros.
-  subst.
+  unfold node.
+  unfold my_specific_tree_rep.
   rewrite -> if_false; eauto.
-  Intros x0 v0 next.
+  Intros x0 v0.
   forward.
-  forward_if. 
+  forward_if. (* if (_x < _y) *)
   - forward. forward. forward.
-    Exists NN next next.
-    unfold extract_node_pn.
-    rewrite H.
+    Exists NN (nextp !!! 0) (nextp !!! 0).
+    unfold node, my_specific_tree_rep.
+    rewrite -> if_false; auto.
+    Exists x0 v0 .
     entailer !.
-    apply elem_of_list_here.
-    unfold node_rep_R.
-    simpl.
-    rewrite -> if_false; eauto.
-    Exists x0 v0 next.
-    entailer !.
-  - forward_if.
+    apply (H8 x). split. lia.
+    auto.
+  - (* if (_x > _y) *)
+    forward_if.
     repeat forward.
-    Exists NF r.1.1.1 n_pt.
-    unfold node_rep_R.
-    simpl.
-    rewrite -> if_false; eauto.
-    Exists x0 v0 next.
+    Exists NF p p.
     entailer !.
+    specialize (H9 x).
+    specialize (H9 H7).
+    specialize (H8 x).
+    apply H8 in H9.
+    destruct H9. lia.
+    unfold node, my_specific_tree_rep.
+    rewrite -> if_false; auto.
+    Exists x0 v0.
+    entailer !.
+    (* x = y *)
     forward.
-    Exists F r.1.1.1 n_pt.
+    Exists F p p.
+    unfold node, my_specific_tree_rep.
+    rewrite -> if_false; auto.
+    Exists x0 v0.
     entailer !.
-    unfold node_rep_R.
-    simpl.
-    rewrite -> if_false; eauto.
-    Exists x0 v0 next.
-    entailer !.
+    assert (x = x0). lia.
+    subst x0.
+    specialize (H8 x).
+    specialize (H9 x).
+    apply H9 in H7.
+    apply H8 in H7. lia.
 Qed.
 
 Definition surely_malloc_spec :=
@@ -125,72 +179,172 @@ Definition surely_malloc_spec :=
        PARAMS (Vptrofs (Ptrofs.repr (sizeof t))) GLOBALS (gv)
        SEP (mem_mgr gv)
     POST [ tptr tvoid ]
-    EX p: _,
+    ∃ p: _,
        PROP ()
        RETURN (p)
-       SEP (mem_mgr gv; malloc_token Ews t p * data_at_ Ews t p).
+       SEP (mem_mgr gv; malloc_token Ews t p; data_at_ Ews t p).
+
+Fixpoint list_to_gmap_aux (l : list Node) (key : nat) : gmap nat Node :=
+  match l with
+  | [] => ∅
+  | x :: xs => <[key:=x]> (list_to_gmap_aux xs (S key))
+  end.
+
+Definition list_to_gmap (l : list Node) : gmap nat Node :=
+  list_to_gmap_aux l 0.
+
+(*  Ip : @flowintT _ K_multiset_ccm  _ _ *)
+
+
 
 Definition insertOp_spec :=
   DECLARE _insertOp
-    WITH x: Z, stt: Z, v: val, p: val, tp: val, l: val, dl: val, next: list val, rng: range,
-                    g: gname, gv: globals
+    WITH x: Z, v: val, stt: Z, p: Node, tp: val, l: val, dl: val,
+                  Ip : @flowintT _ K_multiset_ccm  _ _,
+                    Cp : (gmap Key data_struct.Value),
+                     (* pnext : gmap nat Node, *)
+                      next0: list Node, next: list Node,
+                        sh: share, gv: globals
   PRE [ tptr (tptr t_struct_list), tint, tptr tvoid, tint, tptr (struct_dlist)]
-  PROP (repable_signed x; is_pointer_or_null v; key_in_range x rng = true;
+  PROP (repable_signed x; is_pointer_or_null v; (*node_size = length ((gmap_to_node_list pnext)); *)
+        length next = node_size;
+        (* is_pointer_or_null (Znth 0 (gmap_to_node_list pnext)); *)
         is_pointer_or_null (Znth 0 next);
-        length next = node_size)
+        tp = nullval)
   PARAMS (p; Vint (Int.repr x); v; Vint (Int.repr stt); l)
   GLOBALS (gv)
-  SEP (mem_mgr gv; 
-                     field_at Tsh (struct_dlist) [StructField _list] dl l *
-                     (* field_at Ews (struct_dlist) [StructField _size] (Vptrofs (Ptrofs.repr 2%Z)) l * *)
-                     data_at Ews (tarray (tptr tvoid) (Zlength next)) next dl * 
-                     (* (!!(p = r.1.1.1 /\ p = nullval)  && seplog.emp); *)
-       data_at Ews (tptr t_struct_list) tp p)
+  SEP (mem_mgr gv; node tp Ip Cp (list_to_gmap next0);
+       field_at Tsh (struct_dlist) (DOT _list) dl l;
+       data_at Ews (tptr t_struct_list) tp p;
+                   (* field_at Ews (struct_dlist) [StructField _size] (Vptrofs (Ptrofs.repr 2%Z)) l ∗ *)
+                   (* data_at Ews (tarray (tptr tvoid) (Zlength (gmap_to_node_list pnext) )) (gmap_to_node_list pnext) dl *)
+       data_at Ews (tarray (tptr tvoid) (Zlength next)) next dl
+       )
   POST[ tvoid ]
-  EX (pnt : val),
+  ∃ (pnt : Node),
   PROP (pnt <> nullval)
   LOCAL ()
-  SEP (mem_mgr gv; data_at Ews (tptr t_struct_list) pnt p;
-       node_rep_R pnt (Some (Some (x, v, next))) g;
+  SEP (mem_mgr gv; node pnt Ip (<[x := v]> Cp) (list_to_gmap next);
+       node tp Ip Cp (list_to_gmap next0);
        field_at Tsh struct_dlist (DOT _list) dl l;
-       data_at Ews (tarray (tptr tvoid) (Zlength next)) next dl).
+       data_at Ews (tptr t_struct_list) pnt p;
+       (*data_at Ews (tarray (tptr tvoid) (Zlength (gmap_to_node_list pnext))) (gmap_to_node_list pnext) dl*)
+     data_at Ews (tarray (tptr tvoid) (Zlength next)) next dl  
 
-Lemma length_equal_1 : forall (x: Z) (v: val) (next : list val),
-  length next = 1%nat ->
-  Some (Some (x, v, next)) = Some (Some (x, v, [Znth 0 next])).
-Proof.
-  intros x v next H_length.
-  destruct next as [|a [|b tl]] eqn:Heq_next; try discriminate.
-  inversion H_length; subst.
-  unfold Znth; simpl.
-  repeat f_equal.
-Qed.
+  ).
+
+
 
 Definition Gprog : funspecs :=
     ltac:(with_library prog [acquire_spec; release_spec; makelock_spec;
      surely_malloc_spec; insertOp_spec (* ; traverse_spec; insert_spec; treebox_new_spec*) ]).
 (* Proving insertOp satisfies spec *)
+
 Lemma insertOp: semax_body Vprog Gprog f_insertOp insertOp_spec.
 Proof.
   start_function.
   forward_call (t_struct_list, gv).
+  unfold node, my_specific_tree_rep.
   Intros new_node.
+  clear H5.
+  assert (tp <> nullval). admit.
+  rewrite -> if_false; auto.
   forward.
   forward.
   forward.
   forward.
   entailer !.
-  simpl in H3.
-  rewrite Zlength_correct. lia.
+  rewrite Zlength_correct.
+  simpl in *.
+  rewrite -> H3. lia.
   forward.
   forward.
-  Exists new_node .
-  assert_PROP (new_node <> nullval). entailer !.
-  unfold node_rep_R.
-  unfold my_specific_tree_rep.
+  assert_PROP(new_node ≠ nullval). entailer !.
+  Exists new_node.
+  unfold node, my_specific_tree_rep.
+  rewrite if_false; auto.
+  Intros x0 v0.
+  assert (list_to_gmap_aux next 0 !!! 0 = Znth 0 next).
+  {
+    unfold Znth.
+    destruct next as [| x' xs'].
+    - simpl. auto.
+    - rewrite lookup_total_insert. auto.
+  }
+  rewrite H13.
+  entailer !.
+  Exists x v.
+  rewrite -> if_false; auto.
+  Exists x0 v0.
+  entailer !.
+  entailer !.
+  split. admit.
+  split.
+  intros.
+  split.
+  - intros.
+    split.
+    admit.
+    
+  - 
+    intros.
+    specialize (H5 y).
+    destruct H5.
+    unfold in_outsets in H5. set_solver.
+  - intros.
+    specialize (H5 y).
+    destruct H5.
+    destruct H19.
+    set_solver.
+  - intros.
+    set_solver.
+  Qed.
+
+Lemma insertOp: semax_body Vprog Gprog f_insertOp insertOp_spec.
+Proof.
+  start_function.
+  forward_call (t_struct_list, gv).
+  unfold node, my_specific_tree_rep.
+  Intros new_node.
+  subst.
+  rewrite -> if_true; auto.
+  forward.
+  forward.
+  forward.
+  forward.
+  entailer !.
+  rewrite Zlength_correct.
+  simpl in *.
+  rewrite -> H3. lia.
+  forward.
+  forward.
+  assert_PROP(new_node ≠ nullval). entailer !.
+  Exists new_node.
+  unfold node, my_specific_tree_rep.
   rewrite if_false; auto.
   entailer !.
-  Exists x v (Znth 0 next).
+  Exists x v.
+  assert (list_to_gmap_aux next 0 !!! 0 = Znth 0 next).
+  {
+    unfold Znth.
+    destruct next as [| x' xs'].
+    - simpl. auto.
+    - rewrite lookup_total_insert. auto.
+  }
+  rewrite H18.
   entailer !.
-  by apply length_equal_1.
-Qed.
+  split.
+  intros.
+  split.
+  - intros.
+    specialize (H5 y).
+    destruct H5.
+    unfold in_outsets in H5. set_solver.
+  - intros.
+    specialize (H5 y).
+    destruct H5.
+    destruct H19.
+    set_solver.
+  - intros.
+    set_solver.
+  Qed.
